Reflection/Experiments/ForallTelescope.lean
@@ -1,33 +1,33 @@
-import Reflection.Vec
+import Reflection.Util.Vec
 
-def ForallTelescope (doms : Vec (Sort u) k) (body : ((idx : Fin k) -> Get doms idx) -> Type (max u v)) : Type (max u v) :=
+def ForallTelescope (doms : Vec (Sort u) k) (body : ((idx : Fin k) -> Vec.get doms idx) -> Type (max u v)) : Type (max u v) :=
   match doms with
-  | .nil => body (fun ⟨_, h⟩ => absurd h (Nat.not_lt_zero _))
+  | .nil => body fun ⟨_, h⟩ => absurd h (Nat.not_lt_zero _)
   | .cons A doms' => (x : A) -> ForallTelescope doms' fun f => body fun
     | ⟨0, _h⟩ => x
     | ⟨.succ i, _h⟩ => f ⟨i, _⟩
 
-def ForallTelescopeP (doms : Vec (Sort u) k) (body : ((idx : Fin k) -> Get doms idx) -> Prop) : Prop :=
+def ForallTelescopeP (doms : Vec (Sort u) k) (body : ((idx : Fin k) -> Vec.get doms idx) -> Prop) : Prop :=
   match doms with
-  | .nil => body (fun ⟨_, h⟩ => absurd h (Nat.not_lt_zero _))
-  | .cons A doms' => (x : A) -> ForallTelescopeP doms' (fun f => body (fun
-    | ⟨0, _h⟩ => x
+  | .nil => body (fun ⟨i, h⟩ => absurd h (Nat.not_lt_zero i))
+  | .cons A doms => (x : A) -> ForallTelescopeP doms (fun f => body (fun
+    | ⟨.zero  , _h⟩ => x
     | ⟨.succ i, _h⟩ => f ⟨i, _⟩))
 
 #reduce ForallTelescopeP
-  (Nat ::: String ::: ⟦⟧)
+  (Vec.cons Nat (Vec.cons String .nil))
   (fun f => (f 0 : Nat) = (123 : Nat) /\ f 1 = "Foo")
 
 #reduce ForallTelescopeP
-  (Int ::: String ::: ⟦⟧)
+  (Vec.cons Int (Vec.cons String .nil))
   (fun f => f 1 = f 1 /\ f 0 = f 0)
 
-#reduce ForallTelescope
-  (Type ::: ⟦⟧)
-  (fun f => Vec (f 0) 2)
+-- #reduce ForallTelescope
+--   (Vec.cons Type .nil)
+--   (fun f => Vec (f 0) 2)
 
 #reduce ForallTelescope
-  (ULift.{1, 1} Type ::: ULift.{1, 0} Nat ::: ⟦⟧)
+  (.cons (ULift.{1, 1} Type) <| .cons (ULift.{1, 0} Nat) .nil)
   (fun f => Vec (ULift.down <| f 0) (ULift.down <| f 1))
 
 -- def ForallTelescoper (doms : Vec (Prop -> Prop) k) (body : ((idx : Fin k) -> Get doms idx) -> Sort 0) : Sort 0 :=
