Reflection/Util/EqHelpers.lean
@@ -1,27 +1,27 @@
-import Aesop
+-- import Aesop
 
 -- https://leanprover.zulipchat.com/#narrow/stream/217875-Is-there-code-for-X.3F/topic/.28h.E2.82.82.20.E2.96.B8.20h.E2.82.81.29.20.E2.96.B8.20x.20.3D.20h.E2.82.82.20.E2.96.B8.20.28h.E2.82.81.20.E2.96.B8.20x.29/near/411362225 wow this URL
-@[aesop unsafe]
+-- @[aesop unsafe]
 theorem eq_cast_trans  (h₁ : A = B) (h₂ : B = C) (x : A)
   : h₂ ▸ h₁ ▸ x = (h₂ ▸ h₁) ▸ x
   := by cases h₁; cases h₂; rfl
 
-@[aesop unsafe]
+-- @[aesop unsafe]
 theorem Eq.cast_trans_dep {I} {T : I -> Sort _} {i₁ i₂ i₃ : I} (h₂ : i₂ = i₃) (h₁ : i₁ = i₂) (h₃ : i₁ = i₃) (x : T i₁)
     : h₂ ▸ h₁ ▸ x = h₃ ▸ x
     := by cases h₁; rfl
 
-@[aesop unsafe]
+-- @[aesop unsafe]
 theorem Eq.apply_u {A : T -> Sort _} {f g : (u:T) -> A u} : f = g -> (u : T) -> f u = g u := by
   intro h u; cases h; rfl
 
-@[aesop unsafe]
+-- @[aesop unsafe]
 theorem Eq.cast_apply_u {A : T -> Sort _} {a₁ a₂ : (u:T) -> A u} {h : a₁ = a₂} {hu : (u : T) -> a₁ u = a₂ u}
   {D : (u : T) -> A u -> Sort _} {d₁ : (u : T) -> D u (a₁ u)} {d₂ : (u : T) -> D u (a₂ u)}
   : d₁ = h ▸ d₂ -> (u : T) -> d₁ u = (hu u) ▸ d₂ u := by
   intro ih u; cases h; cases ih; rfl
 
-@[aesop unsafe]
+-- @[aesop unsafe]
 theorem eq_symm_cancel {T : I -> Type u} {a b : I} (h : a = b) (x : T b)
   : h ▸ h.symm ▸ x = x
   := by cases h; rfl
